Weidenbach_Book/IsaSAT_Clauses.thy
@@ -16,6 +16,20 @@ definition length_u where
 definition length_aa_u where
   [simp]: \<open>length_aa_u xs i = length_u (xs ! i)\<close>
 
+definition nth_raa_i_u64 where
+  \<open>nth_raa_i_u64 x L L' = nth_raa x L (nat_of_uint64 L')\<close>
+
+lemma nth_raa_i_uint64_hnr[sepref_fr_rules]:
+  assumes p: \<open>is_pure R\<close>
+  shows
+    \<open>(uncurry2 nth_raa_i_u64, uncurry2 (RETURN \<circ>\<circ>\<circ> nth_rll)) \<in>
+       [\<lambda>((l,i),j). i < length l \<and> j < length_rll l i]\<^sub>a
+       (arlO_assn (array_assn R))\<^sup>k *\<^sub>a nat_assn\<^sup>k *\<^sub>a uint64_nat_assn\<^sup>k \<rightarrow> R\<close>
+  unfolding nth_raa_i_u64_def
+  supply nth_aa_hnr[to_hnr, sep_heap_rules]
+  using assms
+  by sepref_to_hoare (sep_auto simp: uint64_nat_rel_def br_def)
+
 
 named_theorems isasat_codegen \<open>lemmas that should be unfolded to generate (efficient) code\<close>
 
@@ -113,9 +127,41 @@ proof -
     using pre ..
 qed
 
+definition fmap_rll_u64 :: "(nat, 'a literal list \<times> bool) fmap \<Rightarrow> nat \<Rightarrow> nat \<Rightarrow> 'a literal" where
+  [simp]: \<open>fmap_rll_u64  = fmap_rll\<close>
+
+lemma fmap_rll_u64_hnr[sepref_fr_rules]:
+  \<open>(uncurry2 nth_raa_i_u64, uncurry2 (RETURN \<circ>\<circ>\<circ> fmap_rll_u64))
+     \<in> [\<lambda>((N, i), j). i \<in># dom_m N \<and> j < length (N \<propto> i)]\<^sub>a
+     clauses_ll_assn\<^sup>k *\<^sub>a nat_assn\<^sup>k *\<^sub>a uint64_nat_assn\<^sup>k \<rightarrow> unat_lit_assn\<close>
+   (is \<open>_?c\<in> [?pre]\<^sub>a ?im \<rightarrow> ?f\<close>)
+proof -
+  have H:
+    \<open>?c \<in> [comp_PRE (\<langle>Id\<rangle>clauses_l_fmat \<times>\<^sub>f nat_rel \<times>\<^sub>f nat_rel)
+         (\<lambda>((N, i), j). i \<in># dom_m N \<and> j < length (N \<propto> i))
+        (\<lambda>_ ((l, i), j). i < length l \<and> j < length_rll l i)
+         (\<lambda>_. True)]\<^sub>a
+       hrp_comp ((arlO_assn clause_ll_assn)\<^sup>k *\<^sub>a nat_assn\<^sup>k *\<^sub>a uint64_nat_assn\<^sup>k)
+                   (\<langle>Id\<rangle>clauses_l_fmat \<times>\<^sub>f nat_rel \<times>\<^sub>f nat_rel) \<rightarrow> hr_comp unat_lit_assn Id\<close>
+    (is \<open>_ \<in> [?pre']\<^sub>a ?im' \<rightarrow> ?f'\<close>)
+    unfolding fmap_rll_u64_def
+    by (rule hfref_compI_PRE_aux[OF nth_raa_i_uint64_hnr nth_clauses_rll, of unat_lit_assn]) simp
+  have pre: \<open>?pre x \<Longrightarrow> ?pre' x\<close> for x
+    by (auto simp: comp_PRE_def list_fmap_rel_def length_rll_def intro!: ext)
+  have im: \<open>?im' = ?im\<close>
+    unfolding prod_hrp_comp hrp_comp_dest hrp_comp_keep clauses_ll_assn_def
+    by (auto simp: hrp_comp_def hr_comp_def)
+  have f: \<open>?f' = ?f\<close>
+    by auto
+  show ?thesis
+    apply (rule hfref_weaken_pre[OF ])
+     defer
+    using H unfolding f im fmap_rll_u_def apply assumption
+    using pre ..
+qed
+
 definition fmap_length_rll_u :: "(nat, 'a literal list \<times> bool) fmap \<Rightarrow> nat \<Rightarrow> nat" where
   \<open>fmap_length_rll_u l i = length_u (l \<propto> i)\<close>
-
 
 declare fmap_length_rll_u_def[symmetric, isasat_codegen]
 
@@ -140,6 +186,47 @@ proof -
          hr_comp uint32_nat_assn nat_rel\<close>
     (is \<open>_ \<in> [?pre']\<^sub>a ?im' \<rightarrow> ?f'\<close>)
     by (rule hfref_compI_PRE_aux[OF length_raa_u_hnr fmap_length_rll_u, of unat_lit_assn])
+  have pre: \<open>?pre x \<Longrightarrow> ?pre' x\<close> for x
+    by (auto simp: comp_PRE_def list_fmap_rel_def length_rll_def intro!: ext)
+  have im: \<open>?im' = ?im\<close>
+    unfolding prod_hrp_comp hrp_comp_dest hrp_comp_keep clauses_ll_assn_def
+    by (auto simp: hrp_comp_def hr_comp_def)
+  have f: \<open>?f' = ?f\<close>
+    by auto
+  show ?thesis
+    apply (rule hfref_weaken_pre[OF ])
+     defer
+    using H unfolding f im apply assumption
+    using pre ..
+qed
+
+definition fmap_length_rll_u64 :: "(nat, 'a literal list \<times> bool) fmap \<Rightarrow> nat \<Rightarrow> nat" where
+  \<open>fmap_length_rll_u64 l i = length_u (l \<propto> i)\<close>
+
+
+declare fmap_length_rll_u_def[symmetric, isasat_codegen]
+
+(*TODO rename length_rll_n_uint32*)
+lemma fmap_length_rll_u64:
+  \<open>(uncurry (RETURN oo length_rll_n_uint64), uncurry (RETURN oo fmap_length_rll_u64))
+    \<in> [\<lambda>(N, i). i \<in># dom_m N]\<^sub>f \<langle>Id\<rangle>clauses_l_fmat \<times>\<^sub>r nat_rel \<rightarrow> \<langle>nat_rel\<rangle>nres_rel\<close>
+  by (intro frefI nres_relI) (auto simp: list_fmap_rel_def fmap_length_rll_u64_def length_rll_def)
+
+lemma fmap_length_rll_u64_hnr[sepref_fr_rules]:
+  \<open>(uncurry length_raa_u64, uncurry (RETURN \<circ>\<circ> fmap_length_rll_u64))
+     \<in> [\<lambda>(N, i). i \<in># dom_m N \<and> length (N \<propto> i) \<le> uint64_max]\<^sub>a
+     clauses_ll_assn\<^sup>k *\<^sub>a nat_assn\<^sup>k \<rightarrow> uint64_nat_assn\<close>
+   (is \<open>_?c\<in> [?pre]\<^sub>a ?im \<rightarrow> ?f\<close>)
+proof -
+  have H:
+    \<open>?c
+       \<in> [comp_PRE (\<langle>Id\<rangle>clauses_l_fmat \<times>\<^sub>f nat_rel) (\<lambda>(N, i). i \<in># dom_m N)
+            (\<lambda>_ (xs, i). i < length xs \<and> length (xs ! i) \<le> uint64_max)
+            (\<lambda>_. True)]\<^sub>a
+         hrp_comp ((arlO_assn clause_ll_assn)\<^sup>k *\<^sub>a nat_assn\<^sup>k) (\<langle>Id\<rangle>clauses_l_fmat \<times>\<^sub>f nat_rel) \<rightarrow>
+         hr_comp uint64_nat_assn nat_rel\<close>
+    (is \<open>_ \<in> [?pre']\<^sub>a ?im' \<rightarrow> ?f'\<close>)
+    by (rule hfref_compI_PRE_aux[OF length_raa_u64_hnr fmap_length_rll_u64, of unat_lit_assn])
   have pre: \<open>?pre x \<Longrightarrow> ?pre' x\<close> for x
     by (auto simp: comp_PRE_def list_fmap_rel_def length_rll_def intro!: ext)
   have im: \<open>?im' = ?im\<close>
@@ -206,7 +293,7 @@ lemma swap_ll_fmap_swap_ll:
     (auto simp: list_fmap_rel_def Array_List_Array.swap_ll_def)
 
 lemma fmap_swap_ll_hnr[sepref_fr_rules]:
-  \<open>(uncurry3  Array_List_Array.swap_aa, uncurry3 (RETURN oooo fmap_swap_ll))
+  \<open>(uncurry3 swap_aa, uncurry3 (RETURN oooo fmap_swap_ll))
      \<in> [\<lambda>(((N, i), j), k). i \<in># dom_m N \<and> j < length (N \<propto> i) \<and> k < length (N \<propto> i)]\<^sub>a
      clauses_ll_assn\<^sup>d *\<^sub>a nat_assn\<^sup>k *\<^sub>a nat_assn\<^sup>k *\<^sub>a nat_assn\<^sup>k \<rightarrow> clauses_ll_assn\<close>
    (is \<open>?c \<in> [?pre]\<^sub>a ?im \<rightarrow> ?f\<close>)
@@ -234,6 +321,188 @@ proof -
      defer
     using H unfolding f im apply assumption
     using pre ..
+qed
+
+
+
+definition arl_get_u64 :: "'a::heap array_list \<Rightarrow> uint64 \<Rightarrow> 'a Heap" where
+  "arl_get_u64 \<equiv> \<lambda>a i. arl_get' a (integer_of_uint64 i)"
+
+
+lemma arl_get_hnr_u[sepref_fr_rules]:
+  assumes \<open>CONSTRAINT is_pure A\<close>
+  shows \<open>(uncurry arl_get_u64, uncurry (RETURN \<circ>\<circ> op_list_get))
+     \<in> [pre_list_get]\<^sub>a (arl_assn A)\<^sup>k *\<^sub>a uint64_nat_assn\<^sup>k \<rightarrow> A\<close>
+proof -
+  obtain A' where
+    A: \<open>pure A' = A\<close>
+    using assms pure_the_pure by auto
+  then have A': \<open>the_pure A = A'\<close>
+    by auto
+  have [simp]: \<open>the_pure (\<lambda>a c. \<up> ((c, a) \<in> A')) = A'\<close>
+    unfolding pure_def[symmetric] by auto
+  show ?thesis
+    by sepref_to_hoare
+      (sep_auto simp: uint64_nat_rel_def br_def ex_assn_up_eq2 array_assn_def is_array_def
+        hr_comp_def list_rel_pres_length list_rel_update param_nth arl_assn_def
+        A' A[symmetric] pure_def arl_get_u64_def Array.nth'_def arl_get'_def
+        nat_of_uint64_code[symmetric])
+qed
+
+
+definition nth_raa_u64' where
+  \<open>nth_raa_u64' xs x L =  nth_raa xs x (nat_of_uint64 L)\<close>
+
+lemma nth_raa_u'_uint_hnr[sepref_fr_rules]:
+  assumes p: \<open>is_pure R\<close>
+  shows
+    \<open>(uncurry2 nth_raa_u64', uncurry2 (RETURN \<circ>\<circ>\<circ> nth_rll)) \<in>
+       [\<lambda>((l,i),j). i < length l \<and> j < length_rll l i]\<^sub>a
+       (arlO_assn (array_assn R))\<^sup>k *\<^sub>a nat_assn\<^sup>k *\<^sub>a uint64_nat_assn\<^sup>k \<rightarrow> R\<close>
+  supply nth_aa_hnr[to_hnr, sep_heap_rules]
+  using assms
+  by sepref_to_hoare (sep_auto simp: uint64_nat_rel_def br_def nth_raa_u64'_def)
+
+
+definition nth_raa_u64 where
+  \<open>nth_raa_u64 x L =  nth_raa x (nat_of_uint64 L)\<close>
+
+
+lemma nth_raa_uint64_hnr[sepref_fr_rules]:
+  assumes p: \<open>is_pure R\<close>
+  shows
+    \<open>(uncurry2 nth_raa_u64, uncurry2 (RETURN \<circ>\<circ>\<circ> nth_rll)) \<in>
+       [\<lambda>((l,i),j). i < length l \<and> j < length_rll l i]\<^sub>a
+       (arlO_assn (array_assn R))\<^sup>k *\<^sub>a uint64_nat_assn\<^sup>k *\<^sub>a nat_assn\<^sup>k \<rightarrow> R\<close>
+  unfolding nth_raa_u64_def
+  supply nth_aa_hnr[to_hnr, sep_heap_rules]
+  using assms
+  by sepref_to_hoare (sep_auto simp: uint64_nat_rel_def br_def)
+
+definition nth_raa_u64_u64 where
+  \<open>nth_raa_u64_u64 x L L' =  nth_raa x (nat_of_uint64 L) (nat_of_uint64 L')\<close>
+
+
+lemma nth_raa_uint64_uint64_hnr[sepref_fr_rules]:
+  assumes p: \<open>is_pure R\<close>
+  shows
+    \<open>(uncurry2 nth_raa_u64_u64, uncurry2 (RETURN \<circ>\<circ>\<circ> nth_rll)) \<in>
+       [\<lambda>((l,i),j). i < length l \<and> j < length_rll l i]\<^sub>a
+       (arlO_assn (array_assn R))\<^sup>k *\<^sub>a uint64_nat_assn\<^sup>k *\<^sub>a uint64_nat_assn\<^sup>k \<rightarrow> R\<close>
+  unfolding nth_raa_u64_u64_def
+  supply nth_aa_hnr[to_hnr, sep_heap_rules]
+  using assms
+  by sepref_to_hoare (sep_auto simp: uint64_nat_rel_def br_def)
+
+definition update_raa_u64
+   :: "('a::{heap,default}) arrayO_raa \<Rightarrow> nat \<Rightarrow> uint64 \<Rightarrow> 'a \<Rightarrow> 'a arrayO_raa Heap" where
+  \<open>update_raa_u64 a i j y = do {
+      x \<leftarrow> arl_get a i;
+      a' \<leftarrow> heap_array_set_u64 x j y;
+      arl_set a i a'
+    }\<close> -- \<open>is the Array.upd really needed?\<close>
+
+lemma heap_array_set_u64_upd:
+  \<open>heap_array_set_u64 x j xi = Array.upd (nat_of_uint64 j) xi x \<bind> (\<lambda>xa. return x) \<close>
+  by (auto simp:  heap_array_set_u64_def heap_array_set'_u64_def
+     Array.upd'_def nat_of_uint64_code[symmetric])
+
+definition swap_aa_u64  :: "('a::{heap,default}) arrayO_raa \<Rightarrow> nat \<Rightarrow> uint64 \<Rightarrow> uint64 \<Rightarrow> 'a arrayO_raa Heap" where
+  \<open>swap_aa_u64 xs k i j = do {
+    xi \<leftarrow> arl_get xs k;
+    xj \<leftarrow> swap_u64_code xi i j;
+    xs \<leftarrow> arl_set xs k xj;
+    return xs
+  }\<close>
+
+lemma swap_aa_u64_hnr[sepref_fr_rules]:
+  assumes \<open>is_pure R\<close>
+  shows \<open>(uncurry3 swap_aa_u64, uncurry3 (RETURN oooo swap_ll)) \<in>
+   [\<lambda>(((xs, k), i), j). k < length xs \<and> i < length_rll xs k \<and> j < length_rll xs k]\<^sub>a
+  (arlO_assn (array_assn R))\<^sup>d *\<^sub>a nat_assn\<^sup>k *\<^sub>a uint64_nat_assn\<^sup>k *\<^sub>a uint64_nat_assn\<^sup>k \<rightarrow>
+    (arlO_assn (array_assn R))\<close>
+proof -
+  note update_raa_rule_pure[sep_heap_rules]
+  obtain R' where R': \<open>R' = the_pure R\<close> and RR': \<open>R = pure R'\<close>
+    using assms by fastforce
+  have [simp]: \<open>the_pure (\<lambda>a b. \<up> ((b, a) \<in> R')) = R'\<close>
+    unfolding pure_def[symmetric] by auto
+  have H: \<open><is_array_list p (aa, bc) *
+       heap_list_all_nth (array_assn (\<lambda>a c. \<up> ((c, a) \<in> R'))) (remove1 bb [0..<length p]) a p *
+       array_assn (\<lambda>a c. \<up> ((c, a) \<in> R')) (a ! bb) (p ! bb)>
+      Array.nth (p ! bb) (nat_of_integer (integer_of_uint64 bia))
+      <\<lambda>r. \<exists>\<^sub>A p'. is_array_list p' (aa, bc) * \<up> (bb < length p' \<and> p' ! bb = p ! bb \<and> length a = length p') *
+          heap_list_all_nth (array_assn (\<lambda>a c. \<up> ((c, a) \<in> R'))) (remove1 bb [0..<length p']) a p' *
+         array_assn (\<lambda>a c. \<up> ((c, a) \<in> R')) (a ! bb) (p' ! bb) *
+         R (a ! bb ! (nat_of_uint64 bia)) r >\<close>
+    if
+      \<open>is_pure (\<lambda>a c. \<up> ((c, a) \<in> R'))\<close> and
+      \<open>bb < length p\<close> and
+      \<open>nat_of_uint64 bia < length (a ! bb)\<close> and
+      \<open>nat_of_uint64 bi < length (a ! bb)\<close> and
+      \<open>length a = length p\<close>
+    for bi :: \<open>uint64\<close> and bia :: \<open>uint64\<close> and bb :: \<open>nat\<close> and a :: \<open>'a list list\<close> and
+      aa :: \<open>'b array array\<close> and bc :: \<open>nat\<close> and p :: \<open>'b array list\<close>
+    using that
+    by (sep_auto simp: array_assn_def hr_comp_def is_array_def nat_of_uint64_code[symmetric]
+        list_rel_imp_same_length RR' pure_def param_nth)
+  have H': \<open>is_array_list p' (aa, ba) * p' ! bb \<mapsto>\<^sub>a b [nat_of_uint64 bia := b ! nat_of_uint64 bi,
+             nat_of_uint64 bi := xa] *
+      heap_list_all_nth (\<lambda>a b.  \<exists>\<^sub>Aba.  b \<mapsto>\<^sub>a ba *  \<up> ((ba, a) \<in> \<langle>R'\<rangle>list_rel))
+          (remove1 bb [0..<length p']) a p' * R (a ! bb ! nat_of_uint64 bia) xa \<Longrightarrow>\<^sub>A
+      is_array_list p' (aa, ba) *
+      heap_list_all
+       (\<lambda>a c. \<exists>\<^sub>Ab. c \<mapsto>\<^sub>a b *  \<up> ((b, a) \<in> \<langle>R'\<rangle>list_rel))
+       (a[bb := (a ! bb) [nat_of_uint64 bia := a ! bb ! nat_of_uint64 bi,
+             nat_of_uint64 bi := a ! bb ! nat_of_uint64 bia]])
+        p' *  true\<close>
+    if
+      \<open>is_pure (\<lambda>a c. \<up> ((c, a) \<in> R'))\<close> and
+      le: \<open>nat_of_uint64 bia < length (a ! bb)\<close> and
+      le': \<open>nat_of_uint64 bi < length (a ! bb)\<close> and
+      \<open>bb < length p'\<close> and
+      \<open>length a = length p'\<close> and
+      a: \<open>(b, a ! bb) \<in> \<langle>R'\<rangle>list_rel\<close>
+    for bi :: \<open>uint64\<close> and bia :: \<open>uint64\<close> and bb :: \<open>nat\<close> and a :: \<open>'a list list\<close> and
+      xa :: \<open>'b\<close> and p' :: \<open>'b array list\<close> and b :: \<open>'b list\<close> and aa :: \<open>'b array array\<close> and ba :: \<open>nat\<close>
+  proof -
+    have 1: \<open>(b[nat_of_uint64 bia := b ! nat_of_uint64 bi, nat_of_uint64 bi := xa],
+   (a ! bb)[nat_of_uint64 bia := a ! bb ! nat_of_uint64 bi,
+   nat_of_uint64 bi := a ! bb ! nat_of_uint64 bia]) \<in> \<langle>R'\<rangle>list_rel\<close>
+      if \<open>(xa, a ! bb ! nat_of_uint64 bia) \<in> R'\<close>
+      using that a le le'
+      unfolding list_rel_def list_all2_conv_all_nth
+      by auto
+    have 2: \<open>heap_list_all_nth (\<lambda>a b. \<exists>\<^sub>Aba. b \<mapsto>\<^sub>a ba * \<up> ((ba, a) \<in> \<langle>R'\<rangle>list_rel)) (remove1 bb [0..<length p']) a p' =
+    heap_list_all_nth (\<lambda>a c. \<exists>\<^sub>Ab. c \<mapsto>\<^sub>a b * \<up> ((b, a) \<in> \<langle>R'\<rangle>list_rel)) (remove1 bb [0..<length p'])
+     (a[bb := (a ! bb)[nat_of_uint64 bia := a ! bb ! nat_of_uint64 bi, nat_of_uint64 bi := a ! bb ! nat_of_uint64 bia]]) p'\<close>
+      by (rule heap_list_all_nth_cong)  auto
+    show ?thesis using that
+      unfolding heap_list_all_heap_list_all_nth_eq
+      by (subst (2) heap_list_all_nth_remove1[of bb])
+        (sep_auto simp:  heap_list_all_heap_list_all_nth_eq swap_def fr_refl RR'
+          pure_def 2[symmetric] intro!: 1)+
+  qed
+
+  show ?thesis
+    using assms unfolding R'[symmetric] unfolding RR'
+    apply sepref_to_hoare
+
+    apply (sep_auto simp: swap_aa_u64_def swap_ll_def arlO_assn_except_def length_rll_def
+        length_rll_update_rll nth_raa_i_u64_def uint64_nat_rel_def br_def
+        swap_def nth_rll_def list_update_swap swap_u64_code_def nth_u64_code_def Array.nth'_def
+        heap_array_set_u64_def heap_array_set'_u64_def arl_assn_def
+         Array.upd'_def)
+     apply (drule_tac aa = aa and bc =bc in H[of ])
+    apply assumption
+    apply assumption
+    apply assumption
+    apply assumption
+     apply assumption
+    apply (sep_auto simp: array_assn_def nat_of_uint64_code[symmetric] hr_comp_def is_array_def
+        list_rel_imp_same_length arlO_assn_def arl_assn_def hr_comp_def[abs_def])
+    apply (rule H'; assumption?)
+    done
 qed
 
 definition fm_add_new where
@@ -274,7 +543,43 @@ sepref_definition append_and_length_code
 lemma fm_add_new_hnr[sepref_fr_rules]:
   \<open>(uncurry2 append_and_length_code, uncurry2 fm_add_new)
     \<in> bool_assn\<^sup>k *\<^sub>a clause_ll_assn\<^sup>d *\<^sub>a clauses_ll_assn\<^sup>d \<rightarrow>\<^sub>a clauses_ll_assn *a nat_assn\<close>
-  using append_and_length_code.refine[FCOMP append_and_length_fm_add_new] unfolding clauses_ll_assn_def
-  by simp
+  using append_and_length_code.refine[FCOMP append_and_length_fm_add_new]
+  unfolding clauses_ll_assn_def by simp
+
+
+definition fmap_swap_ll_u64 where
+  [simp]: \<open>fmap_swap_ll_u64 = fmap_swap_ll\<close>
+
+lemma fmap_swap_ll_u64_hnr[sepref_fr_rules]:
+  \<open>(uncurry3 swap_aa_u64, uncurry3 (RETURN oooo fmap_swap_ll_u64))
+     \<in> [\<lambda>(((N, i), j), k). i \<in># dom_m N \<and> j < length (N \<propto> i) \<and> k < length (N \<propto> i)]\<^sub>a
+     clauses_ll_assn\<^sup>d *\<^sub>a nat_assn\<^sup>k *\<^sub>a uint64_nat_assn\<^sup>k *\<^sub>a uint64_nat_assn\<^sup>k \<rightarrow> clauses_ll_assn\<close>
+   (is \<open>?c \<in> [?pre]\<^sub>a ?im \<rightarrow> ?f\<close>)
+proof -
+  have H:
+    \<open>?c \<in> [comp_PRE (\<langle>Id\<rangle>clauses_l_fmat \<times>\<^sub>f nat_rel \<times>\<^sub>f nat_rel \<times>\<^sub>f nat_rel)
+             (\<lambda>(((N, i), j), k). i \<in># dom_m N \<and> j < length (N \<propto> i) \<and> k < length (N \<propto> i))
+             (\<lambda>_ (((xs, k), i), j). k < length xs \<and> i < length_rll xs k \<and> j < length_rll xs k)
+             (\<lambda>_. True)]\<^sub>a
+          hrp_comp ((arlO_assn clause_ll_assn)\<^sup>d *\<^sub>a nat_assn\<^sup>k *\<^sub>a uint64_nat_assn\<^sup>k *\<^sub>a uint64_nat_assn\<^sup>k)
+                   (\<langle>Id\<rangle>clauses_l_fmat \<times>\<^sub>f nat_rel \<times>\<^sub>f nat_rel \<times>\<^sub>f nat_rel) \<rightarrow>
+          hr_comp (arlO_assn clause_ll_assn) (\<langle>Id\<rangle>clauses_l_fmat)\<close>
+    (is \<open>_ \<in> [?pre']\<^sub>a ?im' \<rightarrow> ?f'\<close>)
+    unfolding fmap_swap_ll_u64_def
+    by (rule hfref_compI_PRE_aux[OF swap_aa_u64_hnr swap_ll_fmap_swap_ll, of unat_lit_assn]) simp
+  have pre: \<open>?pre x \<Longrightarrow> ?pre' x\<close> for x
+    by (auto simp: comp_PRE_def list_fmap_rel_def length_rll_def intro!: ext)
+  have im: \<open>?im' = ?im\<close>
+    unfolding prod_hrp_comp hrp_comp_dest hrp_comp_keep clauses_ll_assn_def
+    by (auto simp: hrp_comp_def hr_comp_def)
+  have f: \<open>?f' = ?f\<close>
+    unfolding prod_hrp_comp hrp_comp_dest hrp_comp_keep clauses_ll_assn_def
+    by (auto simp: hrp_comp_def hr_comp_def)
+  show ?thesis
+    apply (rule hfref_weaken_pre[OF ])
+     defer
+    using H unfolding f im apply assumption
+    using pre ..
+qed
 
 end
